The example of using packages and existential types is greatly extended. In particular, a development of process scheduling queues is included, as a demonstration of good modularity and information hiding in system design.

examples/HolOmega/packageScript.sml
@@ -96,7 +96,7 @@ val check = eq_ty pkg5_ty pkg6_ty;
 
 (* Using packages *)
 
-fun eval ths tm = QCONV (SIMP_CONV (srw_ss()) ths) tm;
+fun eval ths = QCONV (SIMP_CONV (srw_ss()) ths);
 
 val unpkg5 = ``let (:'x, t:'x # ('x -> num)) = ^pkg5 in (SND t) (FST t)``;
 
@@ -347,6 +347,464 @@ val add2set_th  = save_thm("add2set_th",
 
 val add2bag_th  = save_thm("add2bag_th",
        eval [add2col_def,BAG_CARD_THM,FINITE_BAG_THM] add2bag_tm);
+
+
+(* ------------------------------------------------------------------- *)
+(* The following example is inspired by David Walker's notes for his   *)
+(* Programming Languages course.                                       *)
+(*                                                                     *)
+(* An algorithm for scheduling processes from those ready to run       *)
+(* is represented in two ways: 1) as a list, where newly paused        *)
+(* processes are added to the front, and the next process to run       *)
+(* is selected from the rear, and 2) as a pair of lists, where         *)
+(* new processes are added to the first list at the front, and         *)
+(* where a process to run is removed from the second list at its front *)
+(* unless it is empty, where the second list becomes the reverse of    *)
+(* the first list, and the first list becomes the empty list.          *)
+(*                                                                     *)
+(* The properties that each representation must obey allow are listed  *)
+(* in is_scheduling_q.                                                 *)
+(* ------------------------------------------------------------------- *)
+
+val _ = Hol_datatype
+       `sched_q_opers = <| emptyq : !'b. 'b 'a;
+                           insert : !'b. 'b -> 'b 'a -> 'b 'a;
+                           remove : !'b. 'b 'a -> 'b # 'b 'a;
+                           count  : !'b. 'b -> 'b 'a -> num  |>`;
+
+val is_scheduling_q_def = Define
+   `is_scheduling_q (ops:'a sched_q_opers) =
+      (!:'b. !(x:'b). ops.count x (ops.emptyq[:'b:]) = 0) /\
+      (!:'b. !(q:'b 'a) (x:'b) (y:'b).
+                ops.count x (ops.insert y q) =
+                  if x = y then ops.count x q + 1
+                           else ops.count x q) /\
+      (!:'b. !q:'b 'a.
+              if (!x:'b. ops.count x q = 0) then T else
+                let (y, q') = ops.remove q in
+                !x:'b. ops.count x q = ops.count x (ops.insert y q'))`;
+
+val _ = Hol_datatype
+       `sched_q = <| this : 'b 'a;
+                     ops  : 'a sched_q_opers  |>`;
+
+open listTheory;
+
+val COUNT_DEF = Define
+  `(COUNT (x:'a) [] = 0) /\
+   (COUNT x (y::ys) = if x = y then COUNT x ys + 1
+                               else COUNT x ys)`;
+
+val ALL_COUNT_ZERO = store_thm(
+   "ALL_COUNT_ZERO",
+   ``!xs. (!x:'a. COUNT x xs = 0) = (xs = [])``,
+   Induct
+   THEN REWRITE_TAC [COUNT_DEF]
+   THEN GEN_TAC
+   THEN REWRITE_TAC [NOT_CONS_NIL]
+   THEN CONV_TAC NOT_FORALL_CONV
+   THEN EXISTS_TAC ``h:'a``
+   THEN SIMP_TAC arith_ss []
+  );
+
+val ALL_COUNT_ZERO_2 = store_thm(
+   "ALL_COUNT_ZERO_2",
+   ``!xs ys. (!x:'a. (COUNT x xs = 0) /\ (COUNT x ys = 0)) = (xs = []) /\ (ys = [])``,
+   CONV_TAC (DEPTH_CONV FORALL_AND_CONV)
+   THEN REWRITE_TAC [ALL_COUNT_ZERO]
+  );
+
+val COUNT_LAST = store_thm(
+   "COUNT_LAST",
+   ``!xs. ~(xs = []:'a list) ==>
+          (COUNT (LAST xs) xs = COUNT (LAST xs) (FRONT xs) + 1)``,
+   Induct
+   THEN REWRITE_TAC [NOT_CONS_NIL]
+   THEN GEN_TAC
+   THEN ONCE_REWRITE_TAC [FRONT_DEF]
+   THEN COND_CASES_TAC
+   THENL
+     [ ASM_REWRITE_TAC [COUNT_DEF,LAST_DEF],
+
+       RES_TAC
+       THEN ASM_REWRITE_TAC [COUNT_DEF,LAST_DEF]
+       THEN SRW_TAC [ARITH_ss] []
+     ]
+  );
+
+val COUNT_FRONT = store_thm(
+   "COUNT_FRONT",
+   ``!xs (x:'a). ~(xs = []) ==> ~(x = LAST xs) ==>
+                 (COUNT x (FRONT xs) = COUNT x xs)``,
+   Induct
+   THEN REWRITE_TAC [NOT_CONS_NIL]
+   THEN REPEAT GEN_TAC
+   THEN REWRITE_TAC [FRONT_DEF,LAST_DEF]
+   THEN COND_CASES_TAC
+   THENL
+     [ DISCH_TAC
+       THEN ASM_REWRITE_TAC [COUNT_DEF],
+
+       DISCH_TAC
+       THEN RES_TAC
+       THEN ASM_REWRITE_TAC [COUNT_DEF]
+     ]
+  );
+
+val COUNT_APPEND = store_thm(
+   "COUNT_APPEND",
+   ``!xs ys (x:'a). COUNT x (xs ++ ys) = COUNT x xs + COUNT x ys``,
+   Induct
+   THEN ASM_SIMP_TAC list_ss [COUNT_DEF]
+   THEN REPEAT GEN_TAC
+   THEN COND_CASES_TAC
+   THEN ASM_SIMP_TAC arith_ss []
+  );
+
+val COUNT_REVERSE = store_thm(
+   "COUNT_REVERSE",
+   ``!xs (x:'a). COUNT x (REVERSE xs) = COUNT x xs``,
+   Induct
+   THEN ASM_SIMP_TAC list_ss [COUNT_DEF,COUNT_APPEND]
+   THEN REPEAT GEN_TAC
+   THEN COND_CASES_TAC
+   THEN ASM_SIMP_TAC arith_ss []
+  );
+
+val reference_q_def = Define
+   `reference_q =
+      <| this := [] : num list;
+         ops  := <| emptyq := \:'b. [] : 'b list;
+                    insert := \:'b. \(x:'b) xs. CONS x xs;
+                    remove := \:'b. \xs:'b list. (LAST xs, FRONT xs);
+                    count  := \:'b. \(x:'b) xs. COUNT x xs
+                  |>
+       |>`;
+
+val reference_q_is_scheduling_q = store_thm(
+   "reference_q_is_scheduling_q",
+   ``is_scheduling_q reference_q.ops``,
+   SRW_TAC [ARITH_ss] [reference_q_def,is_scheduling_q_def,COUNT_DEF]
+   THEN REWRITE_TAC [ALL_COUNT_ZERO]
+   THEN STRIP_ASSUME_TAC (ISPEC ``q:'b list`` list_CASES)
+   THEN ASM_REWRITE_TAC [NOT_CONS_NIL]
+   THEN GEN_TAC
+   THEN SIMP_TAC list_ss [GSYM COUNT_LAST]
+   THEN COND_CASES_TAC
+   THEN SRW_TAC [] [COUNT_FRONT]
+  );
+
+val sched_queue_ty = ``:?'a:ty => ty. ('a,num)sched_q``;
+val sched_queue_ty' = ty_antiq sched_queue_ty;
+
+val reference_q_pkg = ``pack(:list, reference_q) : ^sched_queue_ty'``;
+
+(* The following attempt to define REMOVE fails:
+
+val REMOVE_def = Define
+  `(REMOVE (xs:'a list) ([]:'a list) = REMOVE [] (REVERSE xs)) /\
+   (REMOVE xs (y::ys) = (y, (xs,ys)))`;
+
+One way to define REMOVE is by
+
+val REMOVE_defn = Hol_defn "REMOVE"
+  `(REMOVE [] [] = (ARB, ([],[]))) /\
+   (REMOVE (xs:'a list) ([]:'a list) = REMOVE [] (REVERSE xs)) /\
+   (REMOVE xs (y::ys) = (y, (xs,ys)))`;
+
+> val REMOVE_defn =
+    HOL function definition (recursive)
+    
+    Equation(s) :
+     [..]
+    |- REMOVE ([] :α list) ([] :α list) =
+       ((ARB :α),([] :α list),([] :α list))
+     [..]
+    |- REMOVE ((v2 :α)::(v3 :α list)) ([] :α list) =
+       REMOVE ([] :α list) (REVERSE (v2::v3))
+     [..]
+    |- REMOVE ([] :α list) ((y :α)::(ys :α list)) = (y,([] :α list),ys)
+     [..]
+    |- REMOVE ((v4 :α)::(v5 :α list)) ((y :α)::(ys :α list)) = (y,v4::v5,ys)
+    
+    Induction :
+     [..]
+    |- ∀(P :α list -> α list -> bool).
+         P ([] :α list) ([] :α list) ∧
+         (∀(v2 :α) (v3 :α list).
+            P ([] :α list) (REVERSE (v2::v3)) ⇒ P (v2::v3) ([] :α list)) ∧
+         (∀(y :α) (ys :α list). P ([] :α list) (y::ys)) ∧
+         (∀(v4 :α) (v5 :α list) (y :α) (ys :α list). P (v4::v5) (y::ys)) ⇒
+         ∀(v :α list) (v1 :α list). P v v1
+    
+    Termination conditions :
+      0. ∀(v3 :α list) (v2 :α).
+           (R :α list # α list -> α list # α list -> bool)
+             (([] :α list),REVERSE (v2::v3)) (v2::v3,([] :α list))
+      1. WF (R :α list # α list -> α list # α list -> bool)
+     : defn
+
+Then
+
+Defn.tgoal REMOVE_defn;
+e (WF_REL_TAC `measure (\(xs,ys). LENGTH xs)`);
+e (SIMP_TAC list_ss []);
+
+
+val (REMOVE_def,REMOVE_ind) =
+  Defn.tprove (REMOVE_defn,
+    WF_REL_TAC `measure (\(xs,ys). LENGTH xs)`
+    THEN SIMP_TAC list_ss []
+  );
+
+*)
+
+(* from which we can finally create the following definition: *)
+
+val REMOVE_def =
+  tDefine "REMOVE"
+   `(REMOVE [] [] = (ARB, ([],[]))) /\
+    (REMOVE (xs:'a list) ([]:'a list) = REMOVE [] (REVERSE xs)) /\
+    (REMOVE xs (y::ys) = (y, (xs,ys)))`
+  (WF_REL_TAC `measure (\(xs,ys). LENGTH xs)`
+   THEN SIMP_TAC list_ss []);
+
+val REMOVE_ind = theorem "REMOVE_ind";
+
+val REMOVE_CONS = store_thm(
+   "REMOVE_CONS",
+   ``!xs ys (y:'a). REMOVE xs (y::ys) = (y,(xs,ys))``,
+   Cases
+   THEN REWRITE_TAC [REMOVE_def]
+  );
+
+val REVERSE_CONS_NOT_NIL = store_thm(
+   "REVERSE_CONS_NOT_NIL",
+   ``!xs (x:'a). ~(REVERSE (x::xs) = [])``,
+   SIMP_TAC list_ss []
+  );
+
+val REMOVE_COUNT = store_thm(
+   "REMOVE_COUNT",
+   ``!xs ys (u:'a) us vs.
+        (REMOVE xs ys = (u,(us,vs))) ==>
+        ~((xs = []) /\ (ys = [])) ==>
+          !z. COUNT z xs + COUNT z ys =
+              if z = u then COUNT z us + COUNT z vs + 1
+                       else COUNT z us + COUNT z vs``,
+   HO_MATCH_MP_TAC REMOVE_ind
+   THEN REPEAT CONJ_TAC
+   THEN REPEAT GEN_TAC
+   THEN SIMP_TAC list_ss [REMOVE_def,COUNT_DEF,COUNT_APPEND,COUNT_REVERSE]
+   THEN CONV_TAC (RATOR_CONV (ONCE_DEPTH_CONV SYM_CONV))
+   THEN STRIP_TAC
+   THEN GEN_TAC
+   THEN COND_CASES_TAC
+   THEN ASM_SIMP_TAC arith_ss [COUNT_DEF]
+  );
+
+
+val efficient_q_def = Define
+   `efficient_q =
+      <| this := ([] : num list, [] : num list);
+         ops  := <| emptyq := \:'b. ([] : 'b list, [] : 'b list);
+                    insert := \:'b. \x (xs,ys). (CONS x xs, ys);
+                    remove := \:'b. \(xs,ys). REMOVE xs ys;
+                    count  := \:'b. \x (xs,ys). COUNT x xs + COUNT x ys
+                  |>
+       |>`;
+
+val efficient_q_pkg = ``pack(:\'a. 'a list # 'a list, efficient_q)
+                          : ^sched_queue_ty'``;
+
+val check = eq_ty (type_of reference_q_pkg) (type_of efficient_q_pkg);
+
+local open pairLib in end;
+
+val efficient_q_is_scheduling_q = store_thm(
+   "efficient_q_is_scheduling_q",
+   ``is_scheduling_q efficient_q.ops``,
+   SRW_TAC [ARITH_ss] [efficient_q_def,is_scheduling_q_def,COUNT_DEF]
+   THEN REPEAT (POP_ASSUM MP_TAC)
+   THEN PairCases_on `q`
+   THEN SRW_TAC [ARITH_ss] [COUNT_DEF]
+   THEN REWRITE_TAC [ALL_COUNT_ZERO_2]
+   THEN POP_ASSUM MP_TAC
+   THEN Cases_on `q0`
+   THEN Cases_on `q1`
+   THEN PairCases_on `q'`
+   THEN DISCH_TAC
+   THEN IMP_RES_THEN MP_TAC REMOVE_COUNT
+   THEN SRW_TAC [] [COUNT_DEF]
+   THEN COND_CASES_TAC
+   THEN ASM_SIMP_TAC arith_ss []
+  );
+
+(* Implementation of scheduling stack *)
+
+val stack_q_def = Define
+   `stack_q =
+      <| this := [] : num list;
+         ops  := <| emptyq := \:'b. [] : 'b list;
+                    insert := \:'b. \x xs. CONS x xs;
+                    remove := \:'b. \xs. (HD xs,TL xs);
+                    count  := \:'b. \x xs. COUNT x xs
+                  |>
+       |>`;
+
+val stack_q_is_scheduling_q = store_thm(
+   "stack_q_is_scheduling_q",
+   ``is_scheduling_q stack_q.ops``,
+   SRW_TAC [] [stack_q_def,is_scheduling_q_def,COUNT_DEF]
+   THEN Cases_on `q`
+   THEN SRW_TAC [] [COUNT_DEF]
+  );
+
+val stack_q_pkg = ``pack(:list, stack_q) : ^sched_queue_ty'``;
+
+
+(* Operations on scheduling queue packages *)
+
+(* Not allowed:
+
+val thisp_def = Define
+   `thisp (p:^sched_queue_ty') =
+      let (:'a,q) = p in
+        q.this`;
+*)
+
+val insertp_def = Define
+   `insertp i (p:^sched_queue_ty') =
+      let (:'a,q) = p in
+        pack(:'a, <| this := q.ops.insert i q.this;
+                     ops  := q.ops |> )`;
+
+val emptyp_def = Define
+   `emptyp (p:^sched_queue_ty') =
+      let (:'a,q) = p in
+        pack(:'a, <| this := q.ops.emptyq [:num:];
+                     ops  := q.ops |> )`;
+
+val removep_def = Define
+   `removep (p:^sched_queue_ty') =
+      let (:'a,q) = p in
+      let (x,this') = q.ops.remove q.this in
+        (x, pack(:'a, <| this := this';
+                         ops  := q.ops |>))`;
+
+val countp_def = Define
+   `countp i (p:^sched_queue_ty') =
+      let (:'a,q) = p in
+      q.ops.count i q.this`;
+
+val is_scheduling_p_def = Define
+   `is_scheduling_p (p : ?'b. ('b,'a)sched_q) =
+      let (:'a,q) = p in
+      is_scheduling_q q.ops`;
+
+val reference_p_def = Define
+   `reference_p = pack(:list, reference_q) : ^sched_queue_ty'`;
+
+val reference_p_is_scheduling_p = store_thm(
+   "reference_p_is_scheduling_p",
+   ``is_scheduling_p reference_p``,
+   SIMP_TAC bool_ss [is_scheduling_p_def,reference_p_def,reference_q_is_scheduling_q]
+  );
+
+val efficient_p_def = Define
+   `efficient_p = pack(:\'a. 'a list # 'a list, efficient_q) : ^sched_queue_ty'`;
+
+val efficient_p_is_scheduling_p = store_thm(
+   "efficient_p_is_scheduling_p",
+   ``is_scheduling_p efficient_p``,
+   SIMP_TAC bool_ss [is_scheduling_p_def,efficient_p_def,efficient_q_is_scheduling_q]
+  );
+
+val stack_p_def = Define
+   `stack_p = pack(:list, stack_q) : ^sched_queue_ty'`;
+
+val stack_p_is_scheduling_p = store_thm(
+   "stack_p_is_scheduling_p",
+   ``is_scheduling_p stack_p``,
+   SIMP_TAC bool_ss [is_scheduling_p_def,stack_p_def,stack_q_is_scheduling_q]
+  );
+
+val scheduling_p_props = store_thm(
+   "scheduling_p_props",
+   ``!(p: ^sched_queue_ty').
+        is_scheduling_p p ==>
+        (!x. countp x (emptyp p) = 0) /\
+        (!x y. countp x (insertp y p) =
+               if x = y then countp x p + 1
+                        else countp x p) /\
+        (~(!x. countp x p = 0) ==>
+               let (y,p') = removep p
+               in !x. countp x p = countp x (insertp y p'))``,
+   GEN_TAC
+   THEN REWRITE_TAC [is_scheduling_p_def]
+   THEN STRIP_ASSUME_TAC (ISPEC ``p:^sched_queue_ty'`` PACK_ONTO_AX)
+   THEN ASM_REWRITE_TAC []
+   THEN SIMP_TAC bool_ss []
+   THEN REWRITE_TAC [is_scheduling_q_def]
+   THEN REPEAT STRIP_TAC
+   THENL
+     [ SRW_TAC [] [countp_def,emptyp_def],
+
+       SRW_TAC [] [countp_def,insertp_def],
+
+       POP_ASSUM MP_TAC
+       THEN SRW_TAC [] [countp_def,removep_def,insertp_def]
+       THEN FIRST_ASSUM (MP_TAC o Q.SPEC `t.this` o TY_SPEC ``:num``)
+       THEN COND_CASES_TAC
+       THENL
+         [ POP_ASSUM (STRIP_ASSUME_TAC o SPEC ``x:num``),
+
+           SRW_TAC [] [LET_DEF]
+         ]
+     ]
+  );
+
+val emptyp_prop = store_thm(
+   "emptyp_prop",
+   ``!(p: ^sched_queue_ty').
+        is_scheduling_p p ==>
+        !x. countp x (emptyp p) = 0``,
+   SIMP_TAC bool_ss [scheduling_p_props]
+  );
+
+val insertp_prop = store_thm(
+   "insertp_prop",
+   ``!(p: ^sched_queue_ty').
+        is_scheduling_p p ==>
+        !x y. countp x (insertp y p) =
+               if x = y then countp x p + 1
+                        else countp x p``,
+   SIMP_TAC bool_ss [scheduling_p_props]
+  );
+
+val removep_prop = store_thm(
+   "removep_prop",
+   ``!(p: ^sched_queue_ty').
+        is_scheduling_p p ==>
+        ~(!x. countp x p = 0) ==>
+               let (y,p') = removep p
+               in !x. countp x p = countp x (insertp y p')``,
+   SIMP_TAC bool_ss [scheduling_p_props]
+  );
+
+val _ = set_trace "types" 0;
+
+val reference_p_props = save_thm(
+   "reference_p_props",
+   MATCH_MP scheduling_p_props reference_p_is_scheduling_p);
+
+val efficient_p_props = save_thm(
+   "efficient_p_props",
+   MATCH_MP scheduling_p_props efficient_p_is_scheduling_p);
+
+val stack_p_props = save_thm(
+   "stack_p_props",
+   MATCH_MP scheduling_p_props stack_p_is_scheduling_p);
 
 
 val _ = set_trace "types" 1;
